Finish Deref case

compiler/backend/proofs/env_to_stateProofScript.sml
@@ -61,12 +61,14 @@ Inductive compile_rel:
 [~Deref:]
   (compile_rel tl sl ∧ compile_rel ti si ⇒
   compile_rel (Prim (Cons "Deref") [Delay tl; Delay ti])
-              (Lam NONE $ ret (App Sub [si; sl]))) ∧
+              (Lam NONE $ ret (Handle (App Sub [si; sl]) "v"
+                                      (Raise (Delay (Var "v")))))) ∧
 
 [~Update:]
   (compile_rel tl sl ∧ compile_rel ti si ∧ compile_rel tx sx ⇒
   compile_rel (Prim (Cons "Update") [Delay tl; Delay ti; Delay tx])
-              (Lam NONE $ ret (App Update [sl; si; Delay sx]))) ∧
+              (Lam NONE $ ret (Handle (App Update [sl; si; Delay sx]) "v"
+                                      (Raise (Delay (Var "v")))))) ∧
 
 [~Message:]
   (compile_rel te se ⇒
@@ -224,7 +226,8 @@ Inductive v_rel:
      compile_rel tl sl ∧ compile_rel ti si ∧ env_rel tenv senv ⇒
      v_rel
        (Constructor "Deref" [Thunk (INR (tenv,tl)); Thunk (INR (tenv,ti))])
-       (Closure NONE senv (ret (App Sub [si; sl])))) ∧
+       (Closure NONE senv (ret (Handle (App Sub [si; sl]) "v"
+                                       (Raise (Delay (Var "v"))))))) ∧
 
 [~Update:]
   (∀tl sl ti si tx sx tenv senv.
@@ -232,7 +235,8 @@ Inductive v_rel:
      v_rel
        (Constructor "Update"
          [Thunk (INR (tenv,tl)); Thunk (INR (tenv,ti)); Thunk (INR (tenv,tx))])
-       (Closure NONE senv (ret (App Update [sl; si; Delay sx])))) ∧
+       (Closure NONE senv (ret (Handle (App Update [sl; si; Delay sx]) "v"
+                                       (Raise (Delay (Var "v"))))))) ∧
 
 [env_rel:]
   (∀tenv senv.
@@ -863,6 +867,7 @@ Theorem next_thm:
                AppK nenv2 AppOp [Constructor "" []] []::sk ∧
            LIST_REL (LIST_REL v_rel) ts1 ss1)
 Proof
+
   gen_tac \\ completeInduct_on ‘k’
   \\ gvs [PULL_FORALL,AND_IMP_INTRO] \\ rw []
   \\ reverse (Cases_on ‘∃s vs. tv = Constructor s vs’)
@@ -1279,8 +1284,7 @@ Proof
    (reverse (Cases_on ‘LENGTH vs = 2’) >- fs [Once next_def]
     \\ simp [Once v_rel_cases,monad_cns_def]
     \\ strip_tac \\ gvs [with_atoms_def,force_list_def] \\ strip_tac
-    \\ cheat (*
-    \\ ntac 6 (Q.REFINE_EXISTS_TAC ‘ck1+1’ \\ rewrite_tac [step_n_add] \\ fs [step])
+    \\ ntac 7 (Q.REFINE_EXISTS_TAC ‘ck1+1’ \\ rewrite_tac [step_n_add] \\ fs [step])
     \\ rename [‘env_rel tenv senv’]
     \\ pop_assum mp_tac
     \\ once_rewrite_tac [next_def] \\ fs []
@@ -1290,9 +1294,10 @@ Proof
     \\ drule_all eval_thm
     \\ disch_then $ qspecl_then [‘SOME ss’,
                                  ‘AppK senv Sub [] [si]::
-                                  LetK senv (SOME "v")
-                                  (Let (SOME "v") (Delay (Var "v")) (Lam NONE (Var "v")))::
-                                  AppK senv AppOp [Constructor "" []] []::sk’] strip_assume_tac
+               HandleK senv "v" (Raise (Delay (Var "v")))::
+               LetK senv (SOME "v")
+                 (Let (SOME "v") (Delay (Var "v")) (Lam NONE (Var "v")))::
+               AppK senv AppOp [Constructor "" []] []::sk’] strip_assume_tac
     \\ gvs []
     >-
      (first_x_assum $ qspec_then ‘k’ strip_assume_tac \\ fs []
@@ -1303,6 +1308,7 @@ Proof
     \\ drule_all eval_thm
     \\ disch_then $ qspecl_then [‘SOME ss’,
                                  ‘AppK senv Sub [sv] []::
+               HandleK senv "v" (Raise (Delay (Var "v")))::
                LetK senv (SOME "v")
                  (Let (SOME "v") (Delay (Var "v")) (Lam NONE (Var "v")))::
                AppK senv AppOp [Constructor "" []] []::sk’] strip_assume_tac
@@ -1327,7 +1333,86 @@ Proof
     \\ Q.REFINE_EXISTS_TAC ‘ck1+ck'’ \\ rewrite_tac [step_n_add] \\ fs [step]
     \\ gvs [GSYM NOT_LESS]
     \\ Q.REFINE_EXISTS_TAC ‘ck1+1’ \\ rewrite_tac [step_n_add] \\ fs [step]
-    \\ cheat *))
+    \\ gvs [oEL_THM]
+    \\ imp_res_tac LIST_REL_LENGTH \\ gvs []
+    \\ ‘LENGTH (EL n ss) = LENGTH (EL n ts)’ by gvs [listTheory.LIST_REL_EL_EQN]
+    \\ gvs []
+    \\ qpat_x_assum ‘_ ≠ Err’ mp_tac
+    \\ IF_CASES_TAC \\ strip_tac
+    >- (* within bounds case *)
+     (gvs []
+      \\ qabbrev_tac ‘tel = (EL (Num i) (EL n ts))’
+      \\ qabbrev_tac ‘sel = (EL (Num i) (EL n ss))’
+      \\ ‘v_rel tel sel’ by
+       (unabbrev_all_tac
+        \\ qpat_x_assum ‘LIST_REL _ _ _’ mp_tac
+        \\ simp [Once listTheory.LIST_REL_EL_EQN]
+        \\ disch_then drule
+        \\ simp [Once listTheory.LIST_REL_EL_EQN]
+        \\ imp_res_tac integerTheory.NUM_POSINT_EXISTS \\ gvs [])
+      \\ Q.REFINE_EXISTS_TAC ‘ck1+1’ \\ rewrite_tac [step_n_add] \\ fs [step]
+      \\ Q.REFINE_EXISTS_TAC ‘ck1+1’ \\ rewrite_tac [step_n_add] \\ fs [step]
+      \\ Q.REFINE_EXISTS_TAC ‘ck1+1’ \\ rewrite_tac [step_n_add] \\ fs [step]
+      \\ Q.REFINE_EXISTS_TAC ‘ck1+1’ \\ rewrite_tac [step_n_add] \\ fs [step]
+      \\ Q.REFINE_EXISTS_TAC ‘ck1+1’ \\ rewrite_tac [step_n_add] \\ fs [step]
+      \\ Q.REFINE_EXISTS_TAC ‘ck1+1’ \\ rewrite_tac [step_n_add] \\ fs [step]
+      \\ qmatch_goalsub_abbrev_tac ‘Val vvv’
+      \\ first_x_assum $ drule_at $ Pos last
+      \\ fs [LIST_REL_SPLIT1,PULL_EXISTS]
+      \\ rpt (disch_then $ drule_at Any)
+      \\ disch_then (qspecl_then [‘vvv’,‘senv’] mp_tac)
+      \\ impl_tac >-
+       (fs [LIST_REL_REPLICATE_same,Abbr‘vvv’]
+        \\ once_rewrite_tac [v_rel_cases] \\ fs []
+        \\ once_rewrite_tac [v_rel_cases] \\ fs []
+        \\ simp [Once compile_rel_cases,env_rel_def]
+        \\ once_rewrite_tac [v_rel_cases] \\ fs []
+        \\ imp_res_tac LIST_REL_LENGTH \\ fs []
+        \\ gvs [listTheory.LIST_REL_EL_EQN])
+      \\ strip_tac \\ gvs [GSYM PULL_FORALL]
+      \\ qexists_tac ‘n'’ \\ fs [SNOC_APPEND]
+      \\ rename [‘next _ nnn _ mmm’]
+      \\ Cases_on ‘next (k − 1) nnn tk mmm’ \\ gvs [is_halt_def]
+      \\ PairCases_on ‘e’ \\ fs [])
+    (* out of bounds case *)
+    \\ pop_assum mp_tac
+    \\ pop_assum kall_tac \\ gvs [] \\ strip_tac
+    \\ first_x_assum $ drule_at $ Pos last \\ fs []
+    \\ rpt (disch_then $ drule_at $ Pos last)
+    \\ simp [Once v_rel_cases,monad_cns_def]
+    \\ gvs [PULL_EXISTS]
+    \\ simp [Once v_rel_cases,monad_cns_def,PULL_EXISTS]
+    \\ qabbrev_tac ‘aa = next (k − 1) (INR (RaiseVal (Constructor "Subscript" []))) tk ts’
+    \\ simp [Once compile_rel_cases,GSYM PULL_FORALL]
+    \\ rpt (disch_then (qspec_then ‘[("v",Constructor "Subscript" [])] ++ senv’ mp_tac))
+    \\ impl_tac
+    >- (fs [env_rel_def] \\ simp [Once v_rel_cases] \\ fs [monad_cns_def])
+    \\ strip_tac \\ gvs [NOT_LESS]
+    \\ rename [‘step_n nn’] \\ Cases_on ‘nn’ >-
+     (gvs [is_halt_def]
+      \\ Cases_on ‘aa’ \\ fs [] \\ TRY (Cases_on ‘e’ \\ fs []) \\ gvs []
+      \\ qexists_tac ‘0’ \\ fs [is_halt_def])
+    \\ fs [ADD1,step_n_add,step]
+    \\ rename [‘step_n nn’] \\ Cases_on ‘nn’ >-
+     (gvs [is_halt_def]
+      \\ Cases_on ‘aa’ \\ fs [] \\ TRY (Cases_on ‘e’ \\ fs []) \\ gvs []
+      \\ qexists_tac ‘0’ \\ fs [is_halt_def])
+    \\ fs [ADD1,step_n_add,step]
+    \\ rename [‘step_n nn’] \\ Cases_on ‘nn’ >-
+     (gvs [is_halt_def]
+      \\ Cases_on ‘aa’ \\ fs [] \\ TRY (Cases_on ‘e’ \\ fs []) \\ gvs []
+      \\ qexists_tac ‘0’ \\ fs [is_halt_def])
+    \\ fs [ADD1,step_n_add,step]
+    \\ rename [‘step_n nn’] \\ Cases_on ‘nn’ >-
+     (gvs [is_halt_def]
+      \\ Cases_on ‘aa’ \\ fs [] \\ TRY (Cases_on ‘e’ \\ fs []) \\ gvs []
+      \\ qexists_tac ‘0’ \\ fs [is_halt_def])
+    \\ fs [ADD1,step_n_add,step]
+    \\ ntac 9 (Q.REFINE_EXISTS_TAC ‘ck1+1’ \\ rewrite_tac [step_n_add] \\ fs [step])
+    \\ first_x_assum $ irule_at $ Pos hd
+    \\ Cases_on ‘aa’ \\ gvs []
+    \\ PairCases_on ‘e’ \\ gvs [])
+
   \\ Cases_on ‘s = "Update"’ >-
    (reverse (Cases_on ‘LENGTH vs = 3’) >- fs [Once next_def]
     \\ once_rewrite_tac [next_def] \\ fs []
